Split up success and failure

src/Parsers/DependentlyTyped.v
@@ -101,14 +101,8 @@ Section recursive_descent_parser.
 
   Section generic.
     Section parts.
-      Class parser_dependent_types_dataT' `{parser_computational_dataT} :=
-        { (*methods :> parser_computational_dataT;*)
-          T_nonterminal_name_success
-          : forall (str0 : String) (valid : nonterminal_names_listT)
-                   (name : string)
-                   (str : StringWithSplitState String (split_stateT str0 valid (include_nonterminal_name _ name))),
-              Type;
-          T_nonterminal_name_failure
+      Class parser_dependent_types_success_dataT' `{parser_computational_dataT} :=
+        { T_nonterminal_name_success
           : forall (str0 : String) (valid : nonterminal_names_listT)
                    (name : string)
                    (str : StringWithSplitState String (split_stateT str0 valid (include_nonterminal_name _ name))),
@@ -118,15 +112,32 @@ Section recursive_descent_parser.
                    (it : item CharType)
                    (str : StringWithSplitState String (split_stateT str0 valid it)),
               Type;
-          T_item_failure
-          : forall (str0 : String) (valid : nonterminal_names_listT)
-                   (it : item CharType)
-                   (str : StringWithSplitState String (split_stateT str0 valid it)),
-              Type;
           T_production_success
           : forall (str0 : String) (valid : nonterminal_names_listT)
                    (prod : production CharType)
                    (str : StringWithSplitState String (split_stateT str0 valid prod)),
+              Type;
+
+          T_productions_success
+          : forall (str0 : String) (valid : nonterminal_names_listT)
+                   (prods : productions CharType)
+                   (str : StringWithSplitState String (split_stateT str0 valid prods)),
+              Type }.
+
+      Class parser_dependent_types_success_dataT :=
+        { methods :> parser_computational_dataT;
+          stypes' :> parser_dependent_types_success_dataT' }.
+
+      Class parser_dependent_types_failure_dataT' `{parser_dependent_types_success_dataT} :=
+        { T_nonterminal_name_failure
+          : forall (str0 : String) (valid : nonterminal_names_listT)
+                   (name : string)
+                   (str : StringWithSplitState String (split_stateT str0 valid (include_nonterminal_name _ name))),
+              Type;
+          T_item_failure
+          : forall (str0 : String) (valid : nonterminal_names_listT)
+                   (it : item CharType)
+                   (str : StringWithSplitState String (split_stateT str0 valid it)),
               Type;
           T_production_failure
           : forall (str0 : String) (valid : nonterminal_names_listT)
@@ -154,11 +165,6 @@ Section recursive_descent_parser.
                        split)
              -> T_production_failure str0 valid (it::its) str;
 
-          T_productions_success
-          : forall (str0 : String) (valid : nonterminal_names_listT)
-                   (prods : productions CharType)
-                   (str : StringWithSplitState String (split_stateT str0 valid prods)),
-              Type;
           T_productions_failure
           : forall (str0 : String) (valid : nonterminal_names_listT)
                    (prods : productions CharType)
@@ -166,37 +172,22 @@ Section recursive_descent_parser.
               Type }.
 
       Class parser_dependent_types_dataT :=
-        { methods :> parser_computational_dataT;
-          types' :> parser_dependent_types_dataT' }.
+        { stypes :> parser_dependent_types_success_dataT;
+          ftypes' :> parser_dependent_types_failure_dataT' }.
 
-
-      Class parser_dependent_types_extra_dataT' `{types : parser_dependent_types_dataT, @parser_computational_strdataT (@methods types)} :=
-        { (*types :> parser_dependent_types_dataT;
-          strdata :> parser_computational_strdataT;*)
-          lift_success
+      Class parser_dependent_types_extra_success_dataT' `{types : parser_dependent_types_success_dataT, @parser_computational_strdataT (@methods types)} :=
+        { lift_success
           : forall {str0 valid} nonterminal_name {str},
               @T_nonterminal_name_success _ _ str0 valid nonterminal_name (lift_StringWithSplitState str lower_nonterminal_name_state)
               -> @T_item_success _ _ str0 valid (NonTerminal _ nonterminal_name) str;
-          lift_failure
-          : forall {str0 valid} nonterminal_name {str},
-              @T_nonterminal_name_failure _ _ str0 valid nonterminal_name (lift_StringWithSplitState str lower_nonterminal_name_state)
-              -> @T_item_failure _ _ str0 valid (NonTerminal _ nonterminal_name) str;
           parse_terminal_success
           : forall {str0 valid} ch {str},
               let ret := @T_item_success _ _ str0 valid (Terminal ch) str in
               [[ ch ]] =s str -> ret;
-          parse_terminal_failure
-          : forall {str0 valid} ch {str},
-              let ret := @T_item_failure _ _ str0 valid (Terminal ch) str in
-              ([[ ch ]] =s str) = false -> ret;
           parse_empty_success
           : forall {str0 valid str},
               let ret := @T_production_success _ _ str0 valid nil str in
               str =s Empty _ -> ret;
-          parse_empty_failure
-          : forall {str0 valid str},
-              let ret := @T_production_failure _ _ str0 valid nil str in
-              str ≤s str0 -> (str =s Empty _) = false -> ret;
           cons_success
           : forall {str0 valid} it its {s1 s2 str},
               let a1 := @T_item_success _ _ str0 valid it s1 in
@@ -204,8 +195,6 @@ Section recursive_descent_parser.
               let ret := @T_production_success _ _ str0 valid (it::its) str in
               str ≤s str0 -> s1 ++ s2 =s str -> In (s1, s2) (split_string_for_production str0 valid it its str) -> a1 -> a2 -> ret;
 
-          fail_parse_nil_productions
-          : forall {str0 valid str}, T_productions_failure str0 valid [] str;
           lift_prods_success_head
           : forall {str0 valid prod prods str},
               let ret := @T_productions_success _ _ str0 valid (prod::prods) str in
@@ -216,6 +205,38 @@ Section recursive_descent_parser.
               let ret := @T_productions_success _ _ str0 valid (prod::prods) str in
               let arg := @T_productions_success _ _ str0 valid prods (lift_StringWithSplitState str lower_string_tail) in
               arg -> ret;
+
+          lift_parse_nonterminal_name_success_lt
+          : forall {str0 valid nonterminal_name str},
+              let ret := @T_nonterminal_name_success _ _ str0 valid nonterminal_name str in
+              forall (pf : Length str < Length str0),
+                let arg := @T_productions_success _ _ str initial_nonterminal_names_data (Lookup G nonterminal_name) (lift_StringWithSplitState str (lift_lookup_nonterminal_name_state_lt pf)) in
+                arg -> ret;
+          lift_parse_nonterminal_name_success_eq
+          : forall {str0 valid nonterminal_name str},
+              let ret := @T_nonterminal_name_success _ _ str0 valid nonterminal_name str in
+              forall (pf : str = str0 :> String),
+                let arg := @T_productions_success _ _ str0 (remove_nonterminal_name valid nonterminal_name) (Lookup G nonterminal_name) (lift_StringWithSplitState str (lift_lookup_nonterminal_name_state_eq pf)) in
+
+                is_valid_nonterminal_name valid nonterminal_name = true -> arg -> ret
+        }.
+
+      Class parser_dependent_types_extra_failure_dataT' `{types : parser_dependent_types_dataT, @parser_computational_strdataT (@methods (@stypes types))} :=
+        { lift_failure
+          : forall {str0 valid} nonterminal_name {str},
+              @T_nonterminal_name_failure _ _ str0 valid nonterminal_name (lift_StringWithSplitState str lower_nonterminal_name_state)
+              -> @T_item_failure _ _ str0 valid (NonTerminal _ nonterminal_name) str;
+          parse_terminal_failure
+          : forall {str0 valid} ch {str},
+              let ret := @T_item_failure _ _ str0 valid (Terminal ch) str in
+              ([[ ch ]] =s str) = false -> ret;
+          parse_empty_failure
+          : forall {str0 valid str},
+              let ret := @T_production_failure _ _ str0 valid nil str in
+              str ≤s str0 -> (str =s Empty _) = false -> ret;
+
+          fail_parse_nil_productions
+          : forall {str0 valid str}, T_productions_failure str0 valid [] str;
           lift_prods_failure
           : forall {str0 valid prod prods str},
               let ret := @T_productions_failure _ _ str0 valid (prod::prods) str in
@@ -226,25 +247,12 @@ Section recursive_descent_parser.
           H_prod_split : forall str0 valid it its str, split_string_lift_T str0 valid it its str (split_string_for_production str0 valid it its str);
 
 
-          lift_parse_nonterminal_name_success_lt
-          : forall {str0 valid nonterminal_name str},
-              let ret := @T_nonterminal_name_success _ _ str0 valid nonterminal_name str in
-              forall (pf : Length str < Length str0),
-                let arg := @T_productions_success _ _ str initial_nonterminal_names_data (Lookup G nonterminal_name) (lift_StringWithSplitState str (lift_lookup_nonterminal_name_state_lt pf)) in
-                arg -> ret;
           lift_parse_nonterminal_name_failure_lt
           : forall {str0 valid nonterminal_name str},
               let ret := @T_nonterminal_name_failure _ _ str0 valid nonterminal_name str in
               forall (pf : Length str < Length str0),
                 let arg := @T_productions_failure _ _ str initial_nonterminal_names_data (Lookup G nonterminal_name) (lift_StringWithSplitState str (lift_lookup_nonterminal_name_state_lt pf)) in
                 arg -> ret;
-          lift_parse_nonterminal_name_success_eq
-          : forall {str0 valid nonterminal_name str},
-              let ret := @T_nonterminal_name_success _ _ str0 valid nonterminal_name str in
-              forall (pf : str = str0 :> String),
-                let arg := @T_productions_success _ _ str0 (remove_nonterminal_name valid nonterminal_name) (Lookup G nonterminal_name) (lift_StringWithSplitState str (lift_lookup_nonterminal_name_state_eq pf)) in
-
-                is_valid_nonterminal_name valid nonterminal_name = true -> arg -> ret;
           lift_parse_nonterminal_name_failure_eq
           : forall {str0 valid nonterminal_name str},
               let ret := @T_nonterminal_name_failure _ _ str0 valid nonterminal_name str in
@@ -264,7 +272,8 @@ Section recursive_descent_parser.
       Class parser_dependent_types_extra_dataT :=
         { types :> parser_dependent_types_dataT;
           strdata :> parser_computational_strdataT;
-          extradata :> parser_dependent_types_extra_dataT' }.
+          extra_success_data :> parser_dependent_types_extra_success_dataT';
+          extra_failure_data :> parser_dependent_types_extra_failure_dataT' }.
 
       Context `{types_data : parser_dependent_types_extra_dataT}.
 
