src/Parsers/DependentlyTypedSum.v
@@ -91,6 +91,16 @@ Section recursive_descent_parser.
       | inr b => inr (g b)
     end.
 
+  Definition functor_str_sum_type {A B}
+             (f : StringWithSplitState String A -> Type)
+             (g : StringWithSplitState String B -> Type)
+             (x : StringWithSplitState String (fun s => sum (A s) (B s)))
+  : Type
+    := match state_val x with
+         | inl st => f {| state_val := st |}
+         | inr st => g {| state_val := st |}
+       end.
+
   Local Instance sum_strdata : @parser_computational_strdataT _ String G sum_methods
     := { lower_nonterminal_name_state str0 valid nonterminal_name str
          := functor_cross_sum
@@ -121,295 +131,41 @@ Section recursive_descent_parser.
   Variable top_types' : @parser_dependent_types_dataT' _ String top_methods.
   Definition leaf_types' : @parser_dependent_types_dataT' _ String leaf_methods
     := @types' _ _ (@types _ _ _ leaves_extra_data).
+About T_nonterminal_name_success.
+  Local Instance sum_types' : @parser_dependent_types_dataT' _ String sum_methods
+    := { T_nonterminal_name_success str0 valid name
+         := functor_str_sum_type
+              (@T_nonterminal_name_success _ _ _ top_types' _ _ _)
+              (@T_nonterminal_name_success _ _ _ leaf_types' _ _ _);
+         T_nonterminal_name_failure str0 valid name
+         := functor_str_sum_type
+              (@T_nonterminal_name_failure _ _ _ top_types' _ _ _)
+              (@T_nonterminal_name_failure _ _ _ leaf_types' _ _ _);
+         T_item_success str0 valid it
+         := functor_str_sum_type
+              (@T_item_success _ _ _ top_types' _ _ _)
+              (@T_item_success _ _ _ leaf_types' _ _ _);
+         T_item_failure str0 valid it
+         := functor_str_sum_type
+              (@T_item_failure _ _ _ top_types' _ _ _)
+              (@T_item_failure _ _ _ leaf_types' _ _ _);
+         T_production_success str0 valid prod
+         := functor_str_sum_type
+              (@T_production_success _ _ _ top_types' _ _ _)
+              (@T_production_success _ _ _ leaf_types' _ _ _);
+         T_production_failure str0 valid prod
+         := functor_str_sum_type
+              (@T_production_failure _ _ _ top_types' _ _ _)
+              (@T_production_failure _ _ _ leaf_types' _ _ _);
+         T_productions_success str0 valid prods
+         := functor_str_sum_type
+              (@T_productions_success _ _ _ top_types' _ _ _)
+              (@T_productions_success _ _ _ leaf_types' _ _ _);
+         T_productions_failure str0 valid prods
+         := functor_str_sum_type
+              (@T_productions_failure _ _ _ top_types' _ _ _)
+              (@T_productions_failure _ _ _ leaf_types' _ _ _) }.
 
-
-
-  Section minimal.
-    Section parts.
-      Section common.
-        Section types.
-          Context (str0 : String)
-                  (valid : nonterminal_names_listT).
-
-          Let prefix str T := (*size_of_parse_item (ParseNonTerminal name p) < h
-                         ->*) str ≤s str0
-                              -> sub_names_listT is_valid_nonterminal_name valid initial_nonterminal_names_data
-                              -> T.
-
-          Let alt := False (*{ nonterminal_name : string
-                     | is_valid_nonterminal_name initial_nonterminal_names_data nonterminal_name = true
-                       /\ is_valid_nonterminal_name valid nonterminal_name = false }*).
-
-          Section T_nonterminal_name.
-            Context (name : string) (str : StringWithSplitState String (split_stateT str0 valid (include_nonterminal_name _ name))).
-            Let ret := mp_parse_nonterminal_name str0 valid str name.
-
-            Definition T_nonterminal_name_success  : Type
-              := prefix str ret.
-
-            Definition T_nonterminal_name_failure : Type
-              := prefix str match state_val str with
-                              | None => ret -> False
-                              | Some p => alt
-                            end.
-          End T_nonterminal_name.
-
-          Section T_item.
-            Context (it : item CharType) (str : StringWithSplitState String (split_stateT str0 valid it)).
-
-            Let ret := mp_parse_item str0 valid str it.
-
-            Definition T_item_success : Type
-              := prefix str ret.
-            Definition T_item_failure : Type
-              := prefix str match state_val str with
-                              | None => ret -> False
-                              | Some p => alt
-                            end.
-          End T_item.
-
-          Section T_production.
-            Context (prod : production CharType) (str : StringWithSplitState String (split_stateT str0 valid prod)).
-
-            Let ret := mp_parse_production str0 valid str prod.
-
-            Definition T_production_success : Type
-              := prefix str ret.
-            Definition T_production_failure : Type
-              := prefix str match state_val str with
-                              | None => ret -> False
-                              | Some p => alt
-                            end.
-          End T_production.
-
-          Section T_productions.
-            Context (prods : productions CharType) (str : StringWithSplitState String (split_stateT str0 valid prods)).
-
-            Let ret := mp_parse str0 valid str prods.
-
-            Definition T_productions_success : Type
-              := prefix str ret.
-
-            Definition T_productions_failure : Type
-              := prefix str match state_val str with
-                              | None => ret -> False
-                              | Some p => alt
-                            end.
-          End T_productions.
-        End types.
-
-        Global Instance minimal_parser_dependent_types_data
-        : @parser_dependent_types_dataT _ String
-          := {| methods := Build_parser_computational_dataT methods';
-                T_nonterminal_name_success := T_nonterminal_name_success;
-                T_nonterminal_name_failure := T_nonterminal_name_failure;
-                T_item_success := T_item_success;
-                T_item_failure := T_item_failure;
-                T_production_success := T_production_success;
-                T_production_failure := T_production_failure;
-                T_productions_success := T_productions_success;
-                T_productions_failure := T_productions_failure |}.
-
-        Hint Constructors minimal_parse_of minimal_parse_of_name minimal_parse_of_production minimal_parse_of_item unit prod unit : minimal_instance_db.
-        Hint Unfold T_item_success T_item_failure T_production_success T_production_failure T_productions_success T_productions_failure T_nonterminal_name_success T_nonterminal_name_failure
-             DependentlyTyped.T_item_success DependentlyTyped.T_item_failure DependentlyTyped.T_production_success DependentlyTyped.T_production_failure DependentlyTyped.T_productions_success DependentlyTyped.T_productions_failure DependentlyTyped.T_nonterminal_name_success DependentlyTyped.T_nonterminal_name_failure
-             p_parse_production p_parse p_parse_item p_parse_nonterminal_name
-             mp_parse_production mp_parse mp_parse_item mp_parse_nonterminal_name : minimal_instance_db.
-
-        Local Ltac t''0 :=
-          first [ progress cbv zeta
-                | intro
-                (*| progress subst_body*)
-                | let H := (match goal with
-                              | [ H : StringWithSplitState _ _ |- _ ] => constr:H
-                              | [ H : ?T |- _ ] => match eval hnf in T with
-                                                     | StringWithSplitState _ _
-                                                       => constr:H
-                                                   end
-                            end) in
-                  let s := fresh "s" in
-                  let st := fresh "st" in
-                  destruct H as [s st];
-                    change (StringLike.Core.string_val {| string_val := s |}) with s in *;
-                    change (StringLike.Core.state_val {| state_val := st |}) with st in *;
-                    simpl
-                | match goal with
-                    | [ H : option _ |- _ ] => destruct H; simpl
-                    | [ H : ?T |- _ ] => match eval hnf in T with
-                                           | option _ => destruct H; simpl
-                                         end
-                  end
-                | match goal with
-                    | [ H : appcontext[StringLike.Core.string_val {| string_val := ?s |}] |- _ ] => change (StringLike.Core.string_val {| string_val := s |}) with s in *
-                    | [ H : appcontext[StringLike.Core.state_val {| state_val := ?s |}] |- _ ] => change (StringLike.Core.state_val {| state_val := s |}) with s in *
-                  end ].
-
-        Local Ltac t'' :=
-          idtac;
-          match goal with
-            | _ => intro
-            | [ H : False |- _ ] => solve [ destruct H ]
-            | [ H : match _ with _ => _ end |- _ ] => progress hnf in H
-            | _ => solve [ change unit; constructor ]
-            | [ a : _, b : Forall_parse_of_production _ _ |- Forall_parse_of_production _ _ ]
-              => exact (a, b)
-            | [ H : parse_of _ _ _ []  |- _ ] => solve [ exfalso; clear -H; abstract inversion H ]
-            | [ H : {| state_val := Some _ |} = {| state_val := None |} |- _ ]
-              => solve [ destruct (neq_some_none_state_val H) ]
-            | [ H : {| state_val := None |} = {| state_val := Some _ |} |- _ ]
-              => solve [ destruct (neq_some_none_state_val (eq_sym H)) ]
-            | [ H : _ \/ False |- _ ] => apply or_False in H
-            | [ H : _ ≤s _ -> ?B |- _ ] => specialize (H (or_intror eq_refl))
-            | [ H : _ ≤s _ -> ?B, H' : _ \/ _ |- _ ]
-              => first [ specialize (H (transitivity (str_le1_append _ _ _) H'))
-                       | specialize (H (transitivity (str_le2_append _ _ _) H'))
-                       | specialize (H (transitivity split_parse_of_production_le1 H'))
-                       | specialize (H (transitivity split_parse_of_production_le2 H')) ]
-            | [ H : _ ≤s _ -> ?B, H' : _ ≤s _ |- _ ]
-              => first [ specialize (H (transitivity (str_le1_append _ _ _) H'))
-                       | specialize (H (transitivity (str_le2_append _ _ _) H'))
-                       | specialize (H (transitivity split_parse_of_production_le1 H'))
-                       | specialize (H (transitivity split_parse_of_production_le2 H')) ]
-            | [ H : sub_names_listT _ ?x ?y -> _ |- _ ] => specialize (H (reflexivity _))
-            | [ H : sub_names_listT _ _ _, H' : sub_names_listT _ _ _ -> _ |- _ ]
-              => specialize (fun arg => H' (sub_names_listT_remove_2 _ arg _ H))
-            | [ H : context[map _ nil] |- _ ] => progress simpl in H
-            | [ H : context[map _ (_::_)] |- _ ] => progress simpl in H
-            | [ H : appcontext[split_string_for_production _ _ {| state_val := Some _ |} ] |- _ ] => progress simpl in H
-            | _ => progress autounfold with minimal_instance_db in *
-            (*| _ => progress hnf in * *)
-            | [ H : ?T |- _ ] => match head T with
-                                   | match _ with _ => _ end => progress hnf in H
-                                 end
-            | [ |- ?T ] => (not constr_eq False T); solve [ eauto with minimal_instance_db ] (* work around bugged tactic universe successor anomaly *)
-            | [ x : _ |- @sigT ?A _ ]
-              => exists (MinParseNonTerminal x : A)
-            | [ |- @sigT ?A _ ]
-              => first [ (exists (MinParseTerminal _ _ _ _ _ _ _ _ : A))
-                       | (exists (MinParseProductionNil _ _ _ _ _ _ _ : A)) ]
-            | [ x : minimal_parse_of_item _ _ _ _ _ _ _ _ _, y : minimal_parse_of_production _ _ _ _ _ _ _ _ _, H : _ \/ _ |- @sigT ?A _ ]
-              => exists (MinParseProductionCons H x y : A)
-            | [ x : minimal_parse_of_production _ _ _ _ _ _ _ _ _
-                |- @sigT ?A _ ]
-              => exists (MinParseHead _ x : A); assumption
-            | [ x : minimal_parse_of _ _ _ _ _ _ _ _ _
-                |- @sigT ?A _ ]
-              => exists (MinParseTail _ x : A); assumption
-            | [ H : sigT _ |- _ ] => destruct H
-            | [ H : sig _ |- _ ] => destruct H
-            | [ H : prod _ _ |- _ ] => destruct H
-            | [ H : and _ _ |- _ ] => destruct H
-            | [ H : (_, _) = (_, _) |- _ ] => apply path_prod' in H
-            | [ H : ?T |- _ ] => match eval hnf in T with
-                                   | (_ * _)%type => destruct H
-                                   | (_ /\ _)%type => destruct H
-                                 end
-            | _ => progress subst
-            | _ => progress simpl
-            | [ H : _ = _ |- _ ] => progress simpl in H (* work around [simpl in *] causing ~everything, even [admit], to error with "Anomaly: Cannot take the successor of a non variable universe:
-(maybe a bugged tactic).
-Please report." *)
-            | [ H : _ |- _ ] =>
-              match goal with
-                | [ H' : _ = H |- _ ] => destruct H'
-              end
-            | [ H : (_ =s _) = true |- _ ] => apply bool_eq_correct in H
-            | [ H : is_true (_ =s _) |- _ ] => apply bool_eq_correct in H
-            | [ H : parse_of_item _ _ _ (NonTerminal _ _) |- _ ] => (* work around 4035 *) let H' := fresh in rename H into H'; dependent destruction H'
-            | [ H : parse_of_item _ _ _ (Terminal _) |- _ ] => (* work around 4035 *) let H' := fresh in rename H into H'; dependent destruction H'
-            | [ H : parse_of_production _ _ _ [] |- _ ] => (* work around 4035 *) let H' := fresh in rename H into H'; dependent destruction H'
-            | [ H : ?A -> ?B, H' : ?A |- _ ] => specialize (H H')
-            | [ H : ?A -> False |- _ ] => let A' := (eval hnf in A) in progress change (A' -> False) in H
-            | _ => progress trivial
-            | _ => progress auto with arith
-            | _ => t''0
-            | [ H : (_ + _)%type |- _ ] => destruct H
-            | [ |- (_ * _)%type ] => split
-            | [ H : minimal_parse_of_item _ _ _ _ _ _ _ _ (NonTerminal _ _) |- _ ] => (* work around 4035 *) let H' := fresh in rename H into H'; dependent destruction H'
-            | [ H : minimal_parse_of_item _ _ _ _ _ _ _ _ (Terminal _) |- _ ] => (* work around 4035 *) let H' := fresh in rename H into H'; dependent destruction H'
-            | [ H : minimal_parse_of _ _ _ _ _ _ _ _ (_::_) |- _ ] => (* work around 4035 *) let H' := fresh in rename H into H'; dependent destruction H'
-            | [ H : parse_of _ _ _ (_::_) |- _ ] => (* work around 4035 *) let H' := fresh in rename H into H'; dependent destruction H'
-            | [ H : appcontext[if lt_dec ?a ?b then _ else _] |- _ ]
-              => destruct (lt_dec a b)
-          end.
-
-        Local Ltac t' :=
-          first [ t''
-                | match goal with H : true = false |- _ => exfalso; clear -H; congruence end
-                | match goal with H : ?x = false, H' : ?x = true |- _ => exfalso; clear -H H'; abstract congruence end
-                | abstract omega
-                | match goal with H : (?x =s ?x) = false |- _ => erewrite (proj2 (bool_eq_correct _ _ _)) in H by reflexivity end
-                | match goal with H : _ -> False |- False => apply H end;
-                  abstract (repeat t'') ].
-
-        Local Ltac t_false :=
-          idtac;
-          match goal with
-            | [ |- False ]
-              => abstract (
-                     repeat t';
-                     do 2 try inversion_one_head_hnf @minimal_parse_of_name;
-                     repeat t';
-                     do 2 try inversion_one_head_hnf @minimal_parse_of_item;
-                     repeat t';
-                     do 2 try inversion_one_head_hnf @minimal_parse_of_production;
-                     repeat t';
-                     do 2 try inversion_one_head_hnf @minimal_parse_of;
-                     repeat t'
-                   )
-          end.
-
-        Lemma cons_success
-              (str0 : String) (valid : nonterminal_names_listT)
-              (it : item CharType) (its : production CharType)
-              (s1 : StringWithSplitState String (split_stateT str0 valid it))
-              (s2 : StringWithSplitState String (split_stateT str0 valid its))
-              (str : StringWithSplitState String (split_stateT str0 valid (it :: its : production CharType)))
-        : let a1 := DependentlyTyped.T_item_success str0 valid it s1 in
-          let a2 := DependentlyTyped.T_production_success str0 valid its s2 in
-          let ret :=
-              DependentlyTyped.T_production_success str0 valid (it :: its) str in
-          str ≤s str0 ->
-          s1 ++ s2 =s str ->
-          In (s1, s2) (split_string_for_production str0 valid it its str) -> a1 -> a2 -> ret.
-        Proof.
-          destruct str as [ ? [ ] ]; simpl.
-          { intros ? ? H.
-            apply or_False in H.
-            apply path_prod' in H.
-            simpl in H.
-            destruct H as [H' H''].
-            apply neq_some_none_state_val in H'.
-            apply neq_some_none_state_val in H''.
-            simpl in *.
-            repeat t''. }
-          { repeat t''. }
-        Defined.
-
-        Local Ltac t :=
-          repeat t''0;
-          try solve [ repeat t''; exfalso; t_false ].
-
-        Local Obligation Tactic := idtac.
-
-        Definition H_prod_splitT' str0 valid it its str st
-          := split_string_lift_T str0 valid it its {| string_val := str ; state_val := st |} (split_string_for_production str0 valid it its {| string_val := str ; state_val := st |}).
-
-        Lemma H_prod_split_helper str0 valid it its str st
-        : @H_prod_splitT' str0 valid it its str (Some st).
-        Proof.
-          subst_body; simpl in *.
-          intros ? H.
-          simpl in H.
-          destruct_head prod.
-          destruct_head sum;
-            destruct_head prod;
-            unfold T_item_failure, T_production_failure in *;
-            simpl in *.
-          { repeat t''. }
-          { repeat t''. }
-          { repeat t''. }
-        Defined.
 
         Global Program Instance minimal_parser_dependent_types_extra_data
                (H_prod_split' : forall str0 valid it its str, @H_prod_splitT' str0 valid it its str None)
